coq/Named.v
@@ -1,0 +1,91 @@
+Require Import mathcomp.ssreflect.all_ssreflect.
+Set Implicit Arguments.
+Unset Strict Implicit.
+Unset Printing Implicit Defensive.
+Set Bullet Behavior "Strict Subproofs".
+
+From excomp Require Import Exp CoreDefs Core.
+
+Require Import String.
+
+Inductive nexp : Set :=
+| nvar : nat -> nexp
+(* Rule deBruijn index, list of subterms*)
+| ncon : string -> seq nexp -> nexp.
+
+Definition nctx := seq nexp.
+
+(* terms form a category over sorts w/ (empty or constant?) Γ *)
+Inductive named_rule : Type :=
+| nsort : nctx -> string->  named_rule
+| nterm : nctx -> string -> nexp -> named_rule
+| nsort_le : nctx -> nctx -> nexp -> nexp -> named_rule
+| nterm_le : nctx -> nctx -> nexp -> nexp -> nexp -> nexp -> named_rule.
+
+Bind Scope nrule_scope with named_rule.
+Delimit Scope nrule_scope with named_rule.
+Open Scope nrule_scope.
+Notation "{<n c1 <# c2 |- s1 <# s2 }" := (nsort_le c1 c2 s1 s2) (at level 80) : rule_scope.
+Notation "{<n c |- s1 <# s2 }" := (sort_le c c s1 s2) (at level 80):rule_scope.
+Notation "{<n c |- s }" := (sort_le c c s s) (at level 80):rule_scope.
+Notation "{<n c1 <# c2 |- e1 <# e2 .: s1 <# s2 }" :=
+  (nterm_le c1 c2 e1 e2 s1 s2) (at level 80) : rule_scope.
+Notation "{<n c |- e1 <# e2 .: s1 <# s2 }" :=
+  (nterm_le c c e1 e2 s1 s2) (at level 80) : rule_scope.
+Notation "{<n c |- e1 <# e2 .: s }" :=
+  ({<n c |- e1 <# e2 .: s <# s}) (at level 80) : rule_scope.
+Notation "{<n c |- e .: s }" := 
+  ({< c |- e <# e.: s}) (at level 80) : rule_scope.
+Notation "{|n c |- name 'sort' }" := 
+  (nsort c name) (at level 80) : rule_scope.
+Notation "{|n c |- name .: s }" := 
+  (nterm c name s) (at level 80) : rule_scope.
+
+Fixpoint idx (l : seq string) (a : string) : nat :=
+  match l with
+  | [::] => 0
+  | a'::l' => if eqb a a' then 0 else (idx l' a).+1
+  end.
+
+Fixpoint index_named_exp nl (e : nexp) : exp :=
+  match e with
+  | nvar n => var n
+  | ncon s l => con (idx nl s) (map (index_named_exp nl) l)
+  end.
+
+Definition index_named_rule nl (r : named_rule) : rule :=
+  match r with
+  | {|n c |- nm sort } => {| map (index_named_exp nl) c |- sort }
+  | {|n c |- nm .: s } => {| map (index_named_exp nl) c |- index_named_exp nl s }
+  | {<n c1 <# c2 |- s1 <# s2 } =>
+    {< map (index_named_exp nl) c1
+           <# map (index_named_exp nl) c2
+     |- index_named_exp nl s1 <# index_named_exp nl s2}
+  | {<n c1 <# c2 |- e1 <# e2 .: s1 <# s2 } =>
+    {< map (index_named_exp nl) c1
+           <# map (index_named_exp nl) c2
+     |- index_named_exp nl e1 <# index_named_exp nl e2
+    .: index_named_exp nl s1 <# index_named_exp nl s2}
+  end.
+
+Definition name_of (r : named_rule) : string :=
+  match r with
+  | {|n c |- nm sort } => nm
+  | {|n c |- nm .: s } => nm
+  | {<n c1 <# c2 |- s1 <# s2 } => "@#!$"
+  | {<n c1 <# c2 |- e1 <# e2 .: s1 <# s2 } => "@#!$"
+  end.
+
+Fixpoint index_nlang' (nl : seq string) (l : seq named_rule) : lang * seq string :=
+  match l with
+  | [::] => ([::],[::])
+  | r :: l' =>
+    let (lout,nl') := index_nlang' nl l' in
+    let rout := index_named_rule nl' r in
+    let rn := name_of r in
+    (rout::lout, rn::nl')
+  end.
+
+Definition index_nlang l :=
+  let (lout,_):= index_nlang' [::] l in
+  lout.
